\begin{definition}
Let $Th(\MMM) =  \{\phi\ |\ \MMM \models \phi \}$.
\end{definition}

\begin{theorem}
\[
\MMM' \MODELLEQ \MMM
\qquad\text{iff}\qquad
Th(\MMM) \subseteq Th(\MMM') .
\]
\end{theorem}

\begin{proof}
\begin{case}
First, left to right
\end{case}
Assume $\MMM' \MODELLEQ \MMM$ and $\MMM \models \phi$.
We must show $\MMM' \models \phi$.
Let $\MMM = (\LLL, w)$ and $\MMM' = (\LLL', w')$.
The proof proceeds by induction on $\phi$.
The cases for $\top$ and $\land$ are trivial.

Assume $\phi = \MAY{a}\psi$ and assume  $(\LLL, w) \models  \MAY{a}\psi$.
Then $w \xrightarrow{a} x$ and $(\LLL, x) \models  \psi$.
As $\MMM'$ simulates $\MMM$, there is an $x'$ such that $(x,x') \in R$ and $w' \xrightarrow{a} x'$.
By the induction hypothesis, $(\LLL', x') \models \psi$.
Therefore, by the semantic clause for $!$, $(\LLL', w') \models  \MAY{a}\psi$.

Assume now that $\phi = \; ! \; A$, for some finite $A \subseteq \Sigma$, and that $(\LLL, w) \models \; ! \; A$.
By the semantic clause for $!$, $\lambda(w) \subseteq A$.
Since $(\LLL', w') \MODELLEQ (\LLL, w)$, by the definition of simulation of eremic transition systems, $\lambda(w) \supseteq \lambda'(w')$.
Therefore, $\lambda'(w') \subseteq \lambda(w) \subseteq A$.
Therefore, by the semantic clause for $!$, $(\LLL', w') \models  \; ! \; A$.

\begin{case}
Second, right to left.
\end{case}
Let $\MMM = (\LLL, w)$ and $\MMM' = (\LLL', w')$.
Assume $Th(\MMM) \subseteq Th(\MMM') $. We need to show that $\MMM'$ simulates $\MMM$.
In other words, we need to produce a relation $R \subseteq \mathcal{W} \times \mathcal{W}'$ where $(w,w') \in R$ and $R$ is a simulation from $(\LLL, w)$ to $ (\LLL', w')$.
Define $R = \{(x,x') \; | \; Th( (\LLL, x)) \subseteq Th( (\LLL', x'))\}$.
Clearly, $(w,w') \in R$, as $Th((\LLL, w)) \subseteq Th((\LLL', w')) $.
To show that $R$ is a simulation,  assume $x \xrightarrow{a} y$ in $\LLL$ and $(x,x') \in R$. We need to provide a $y'$ such that $x' \xrightarrow{a} y'$ in $\LLL'$.
Consider the formula $\MAY{a}\top$. Now $(\LLL, x) \models \MAY{a}\top$ because $x \xrightarrow{a} y$.
But as $(x,x') \in R$, $Th((\LLL, x)) \subseteq Th((\LLL', x')) $, so  $(\LLL', x') \models \MAY{a}\top$.
But, by the semantic clause for $\MAY{a}$, this means there is a $y'$ such that $x' \xrightarrow{a} y'$ in $\LLL'$,

Finally, we need to show that whenever $(x,x') \in R$, then $\lambda(x) \supseteq \lambda'(x')$.
Assume, first, that $\lambda(x)$ is finite. 
Then $(\LLL, x) \models \; ! \; \lambda(x)$.
But as $(x,x') \in R$, $Th((\LLL, x)) \subseteq Th((\LLL', x')) $, so  $(\LLL', x') \models \; ! \; \lambda(x)$.
But, by the semantic clause for $!$, $(\LLL', x') \models \; ! \; \lambda(x)$ iff $\lambda'(x') \subseteq \lambda(x)$.
Therefore $\lambda(x) \supseteq \lambda'(x')$.
If, on the other hand, $\lambda(x)$ is infinite, then $\lambda(x) = \Sigma$ (because the only infinite node labelling that we allow is $\Sigma$). Every node labelling is a subset of $\Sigma$, so in this case too, $\lambda(x) = \Sigma \supseteq \lambda'(x')$.


\end{proof}
